# Radical Equations

## Design a Pendulum clock

::::: {.rmdthink}

:::: {.twocols}

::: {.pullleft}

A pendulum clock is a clock that uses a pendulum, a swinging weight, as its timekeeping element. [Galileo Galilei](https://en.wikipedia.org/wiki/Galileo_Galilei) discovered in early 17th century the relation between the length $L$ of a pendulum and the period $T$ of th pendulum. For a pendulum clock, the relations is approximately determined by the following [rule of thumb formula](https://en.wikipedia.org/wiki/Pendulum_(mathematics)):
$$
T\approx 2\sqrt{L}
$$
given that $L$ and $T$ are measured in meters and seconds respectively. If the period of a pendulum clock is 2 seconds, how long should be the pendulum?

:::

::: {.pullright style="vertical-align: middle;"}

```{r echo=FALSE, include=knitr::is_latex_output()}

if (knitr::is_latex_output()) {
    knitr::opts_chunk$set(out.width="50%")
    knitr::include_graphics("figs/pendulum-clock.pdf")
}

```

```{r echo=FALSE, include=knitr::is_html_output()}

    knitr::include_graphics("figs/pendulum-clock.gif")

```

:::

::::

:::::

<!--
## Why is The Square Root of Two Irrational

```{block2, type="rmdthink"}

We know that the number $\sqrt{2}$ is not a rational number. But why? Can you give an explanation?

[^square]: Watch the youtube video <https://www.youtube.com/watch?v=f1yDExNAEMg> for interesting explanation.

```
-->

## Solving Radical Equations by Taking a Power

The idea to solve a radical equation $\sqrt[n]{X}=a$ is to first take $n$-th power of both sides to get rid of the radical sign, that is $X=a^n$ and then solve the resulting equation.

::: {.rmdtip}

**Solve by Reduction**  
The goal to solve a single variable equation is to isolate the variable. When an equation involves radical expressions, you can not isolate the variable arithmetically without eliminating the radical sign unless the radicand is a perfect power. To remove a radical sign, you make take a power. However, you'd better to isolate it first. Because simply taking powers of both sides may create new radical expressions.

:::

```{example}

Solve the equation $x-\sqrt{x+1}=1.$

```

```{solution}
\

1. Arrange terms so that one radical is isolated on one side of the equation.
   $$x-1=\sqrt{x+1}$$
1. Square both sides to eliminate the square root.
   $$(x-1)^2=x+1$$
1. Solve the resulting equation.
   $$
      \begin{aligned}
          x^2-2x+1&=x+1\\
          x^2-3x&=0\\
          x(x-3)&=0
      \end{aligned}
   $$
   $$
   \begin{aligned}
      x =0 & \qquad \text{or} & x-3 =0 \\
      x =0 & \qquad \text{or} & x   =3
   \end{aligned}
   $$
1. Check all proposed solutions.  
   Plug $x=0$ into the original equation, we see that the left hand side is  $0-\sqrt{0+1}=0-\sqrt{1}=0-1=-1$ which is not equal to the right hand side. So $x=0$ cannot be a solution.

   Plug $x=3$ into the original equation, we see that the left hand side is $3-\sqrt{3+1}=3-\sqrt{4}=3-2=1$. So $x=3$ is a solution.

```

```{example}

Solve the equation $\sqrt{x-1}-\sqrt{x-6}=1.$

```

```{solution}
\

1. Isolated one radical.
   $$
      \sqrt{x-1}=\sqrt{x-6}+1\\
   $$
1. Square both sides to remove radical sign and then isolate the remaining radical.
   $$
      \begin{aligned}
          x-1&=(x-6)+2\sqrt{x-6}+1\\
          x-1&=x-5+2\sqrt{x-6}\\
          4&=2\sqrt{x-6}\\
          2&=\sqrt{x-6}.
      \end{aligned}
   $$
1. Square both sides to remove the radical sign and then solve.
   $$
      \begin{aligned}
          \sqrt{x-6}&=2\\
          x-6&=4\\
          x&=10.
      \end{aligned}
   $$
   Since $10-1>0$ and $10-6>0$, $x=10$ is a valid solution. Indeed,
   $$
      \sqrt{10-1}-\sqrt{10-6}=\sqrt{9}-\sqrt{4}=3-2=1.
   $$

```

```{example}

Solve the equation $-2\sqrt[3]{x-4}=6.$

```

```{solution}
\

1. Isolated the radical.
   $$
      \sqrt[3]{x-4}=-3
   $$
2. Cube both sides to eliminate the cube root and then solve the resulting equation.
   $$
      \begin{aligned}
          x-4&=(-3)^3\\
          x-4&=-27\\
          x&=-23
      \end{aligned}
   $$
   The solution is $x=-23$.

```

## Equations Involving Rational Exponents

Equation involving rational exponents may be solved similarly. However, one should be careful with meaning of the expression $\left(X^{\frac mn}\right)^{\frac nm}$. When $m$ is even and $n$ is odd, $\left(X^{\frac mn}\right)^{\frac nm}=|X|$. Otherwise, $\left(X^{\frac mn}\right)^{\frac nm}=X$.

```{example}

Solve the equation $(x+2)^{\frac12}-(x-3)^{\frac12}=1$.

```

```{solution}
\

Since there are more than one term involving rational exponents, to solve the equation, we isolate one term and taking power and so on so forth.
$$
\begin{aligned}
    (x+2)^{\frac12}-(x-3)^{\frac12}=&1\\
    (x+2)^{\frac12}=& (x-3)^{\frac12}+1\\
    x+2 =& \left((x-3)^{\frac12}+1\right)^2\\
    x+2 =& (x-3)+2(x-3)^{\frac12}+1\\
    2(x-3)^{\frac12}=&4\\
    (x-3)^{\frac12}=&2\\
    x-3=&4\\
    x=&7
\end{aligned}
$$
Check:
$$(7+2)^{\frac12}-(7-3)^{\frac12}=\sqrt{9}-\sqrt{4}=3-2=1.$$

So the equation has one solution $x=7$.

```

```{example}

Solve the equation $(x-1)^{\frac{2}{3}}=4$.

```

```{solution}
\

There are different way to solve this equation. One may is to take rational powers of both sides and solve the resulting equation.
$$
\begin{aligned}
    (x-1)^{\frac{2}{3}}=&4\\
    \left((x-1)^{\frac{2}{3}}\right)^{\frac32}=&4^{\frac32}\\
    |x-1|=&8\\
    x-1=8 \qquad\text{or}&\qquad x-1=-8\\
    x=9 \qquad\text{or}&\qquad x=-7
\end{aligned}
$$
Check:
$$(9-1)^{\frac23}=8^{\frac23}=(8^{\frac13})^2=2^2=4;$$
$$(-7-1)^{\frac23}=(-8)^{\frac23}=((-8)^{\frac13})^2=(-2)^2=4.$$

So the equation has two solutions $x=9$ and $x=-7$.

```

## Learn from Mistakes

```{example}

Can you find the mistakes made in the solution and fix it?

Solve the radical equation.
$$\sqrt{x-1}+2=x$$

<div style="color: red">
**Solution (incorrect)**:
$$
\begin{aligned}
\sqrt{x-2}+2&=x\\
(\sqrt{x-2})^2+2^2&=x^2\\
x-2+4&=x^2\\
x+2&=x^2\\
x^2-x-2&=0\\
(x-2)(x+1)&=0\\
x-2=0 \qquad\text{or}& \qquad x+1=0\\
x=2 \qquad\text{or}&\qquad x=-1
\end{aligned}
$$
Answer: the equation has two solutions $x=2$ and $x=-1$.
</div>

```

```{solution}
\

When squaring one side of the equation, the other side as a whole should be squared. The mistake occurred at the squaring step. The right way to solve the equation is as follows.
$$
\begin{aligned}
\sqrt{x-2}+2&=x\\
\sqrt{x-2}&=x-2\\
x-2&=(x-2)^2\\
(x-2)^2-(x-2)&=0\\
(x-2)(x-2-1)&=0\\
(x-2)(x-3)&=0\\
x=2 \qquad\text{or}&\qquad x=3
\end{aligned}
$$
Because squaring is not an equivalent transformation in general, the solutions of the resulting equations must be checked. When $x=2$, the left side of the original equation is $\sqrt{2-2}+2=0+2=2$. When $x=3$, the left side is $\sqrt{3-2}+2=1+2=3$. So both $x=2$ and $x=3$ are solutions of the function $\sqrt{x-1}+2=x$.

```

\newpage

## Practice

```{exercise}

Solve each radical equation.

1. $\sqrt{3x+1}=4$
1. $\sqrt{2x-1}-5=0$


```

```{exercise}

Solve each radical equation.

1. $\sqrt{5x+1}=x+1$
1. $x=\sqrt{3x+7}-3$

```

```{exercise}

Solve each radical equation.

1. $\sqrt{6x+7}-x=2$
1. $\sqrt{x+2}+\sqrt{x-1}=3$

```

```{exercise}

Solve each radical equation.

1. $\sqrt{x+5}-\sqrt{x-3}=2$
1. $3\sqrt[3]{3x-1}=6$

```

```{exercise}

Solve each radical equation.

1. $(x+3)^{\frac12}=x+1$
1. $2(x-1)^{\frac12}-(x-1)^{-\frac12}=1$

```

```{exercise}

Solve each radical equation.

1. $(x-1)^{\frac32}=8$
1. $(x+1)^{\frac23}=4$

```
